---
layout: page
title: Problem Paper 6 — Solutions
permalink: /courses/math-1115/problem-paper-solutions/pp6/
---

# MATH 1115 — Problem Paper 6: Solutions
<!-- KaTeX: load once per page/layout -->
<link rel="stylesheet" href="https://cdn.jsdelivr.net/npm/katex@0.16.11/dist/katex.min.css" integrity="sha384-3UiQGuEI4TTMaFmGIZumfRPtfKQ3trwQE2JgosJxCnGmQpL/lJdjpcHkua0MUl+0" crossorigin="anonymous">
<script defer src="https://cdn.jsdelivr.net/npm/katex@0.16.11/dist/katex.min.js" integrity="sha384-3zX+qC0xOeQ0l8q0kAO2J3oBv7z1o2w4v7YH7pH6xCwG8g7k3+7O9v/0ZqU3H2wM" crossorigin="anonymous"></script>
<script defer src="https://cdn.jsdelivr.net/npm/katex@0.16.11/dist/contrib/auto-render.min.js" integrity="sha384-mll67QQbWIoF4Fvb8nL7+8bX2f+v8DkKf9g6Xv5U0b8k2iTq2n7QqN2U6E9mlUQK" crossorigin="anonymous"
        onload="renderMathInElement(document.body,{delimiters:[{left:'$$',right:'$$',display:true},{left:'\\(',right:'\\)',display:false}]});"></script>


<details open>
  <summary><strong>Q4(a)</strong> — Solve the system</summary>

  <h4>Given</h4>
  <p>
    $$\begin{aligned}
      3x - 2y &= 7 \quad &(1)\\
      -\tfrac{3}{2}x + y &= 5 \quad &(2)
    \end{aligned}$$
  </p>

  <h4>Step 1: Make \(y\) the subject of (2)</h4>
  <p>
    $$y = \tfrac{3}{2}x + 5 \quad (3)$$
  </p>

  <h4>Step 2: Substitute (3) into (1)</h4>
  <p>
    $$\begin{aligned}
      3x - 2\!\left(\tfrac{3}{2}x + 5\right) &= 7 \\
      3x - 3x - 10 &= 7 \\
      -10 &= 7
    \end{aligned}$$
  </p>

  <p><strong>Conclusion:</strong> \(-10=7\) is a contradiction, so the system has <strong>no solution</strong>.</p>
</details>








<details open>
  <summary><strong>Q4(b)</strong> — Solve the system</summary>

  <h4>Given</h4>
  <p>
    $$\begin{aligned}
      5y - 2x &= -2 \quad &(1)\\
      4x - 10y &= 4 \quad &(2)
    \end{aligned}$$
  </p>

  <h4>Step 1: Multiply equation (1) by 2</h4>
  <p>
    $$10y - 4x = -4 \quad (3)$$
  </p>

  <h4>Step 2: Compare equations (2) and (3)</h4>
  <p>
    $$\begin{cases}
      -4x + 10y = -4 \\
      4x - 10y = 4
    \end{cases}$$
  </p>

  <p>
    Notice that equation (3) is a scalar multiple of equation (2).  
    Hence, the two equations are <strong>dependent</strong>; they represent the same line.
  </p>

  <p><strong>Conclusion:</strong> There are infinitely many solutions.</p>
</details>




<details open>
  <summary><strong>Q4(c)</strong> — Solve the system</summary>

  <h4>Given</h4>
  <p>
    $$\begin{aligned}
      2x + y &= 1 \quad &(1)\\
      3x + 4y &= 14 \quad &(2)
    \end{aligned}$$
  </p>

  <h4>Step 1: Multiply (1) by 4</h4>
  <p>
    $$8x + 4y = 4 \quad (3)$$
  </p>

  <h4>Step 2: Eliminate \(y\) using (3) − (2)</h4>
  <p>
    $$\begin{aligned}
      (8x + 4y) - (3x + 4y) &= 4 - 14 \\
      5x &= -10 \\
      x &= -2
    \end{aligned}$$
  </p>

  <h4>Step 3: Substitute \(x=-2\) into (2)</h4>
  <p>
    $$\begin{aligned}
      3(-2) + 4y &= 14 \\
      -6 + 4y &= 14 \\
      4y &= 20 \\
      y &= 5
    \end{aligned}$$
  </p>

  <p><strong>Conclusion:</strong> The solution is \(\boxed{(x,y)=(-2,\,5)}\).</p>
</details>



<details open>
  <summary><strong>Q4(d)</strong> — Solve the system</summary>

  <h4>Given</h4>
  <p>
    $$\begin{aligned}
      3x + 2y &= 14 \quad &(1)\\
      x - 2y &= 2 \quad &(2)
    \end{aligned}$$
  </p>

  <h4>Step 1: Add equations (1) and (2)</h4>
  <p>
    $$\begin{aligned}
      (3x + 2y) + (x - 2y) &= 14 + 2 \\
      4x &= 16 \\
      x &= 4
    \end{aligned}$$
  </p>

  <h4> Substitute \(x = 4\) into (2)</h4>
  <p>
    $$\begin{aligned}
      4 - 2y &= 2 \\
      -2y &= -2 \\
      y &= 1
    \end{aligned}$$
  </p>

  <p><strong>Conclusion:</strong> The solution is \(\boxed{(x, y) = (4,\,1)}\).</p>
</details>



<a class="btn" href="{{ '/courses/math-1115/problem-paper-solutions/' | relative_url }}">← Back to Problem Paper Solutions</a>
&nbsp;
<a class="btn" href="{{ '/courses/math-1115/problem-paper-solutions/pp6/pp6-solutions.pdf' | relative_url }}">Download PDF</a>

